CompCert/EventsInform.v
@@ -1,6 +1,7 @@
 Require Import Common.Definitions.
 Require Import Common.Values.
 Require Import CompCert.Coqlib.
+Require Import CompCert.Events.
 
 (* RB: TODO: RW: Allowing arbitrary values to appear in events does not preclude
    the possibility of nonsensical values appearing in traces, notably Undef
@@ -8,12 +9,10 @@ Require Import CompCert.Coqlib.
     1. Rule out Undef values in the semantics.
     2. Refine the definition of defined and undefined values at the type level.
 *)
-Inductive event :=
-| ECall : Component.id -> Procedure.id -> Z (* value *) -> Component.id -> event
-| ERet : Component.id -> Z (* value *) -> Component.id -> event
-| ERead : Component.id -> Pointer.t -> value -> event
-| EWrite : Component.id -> Pointer.t -> value -> event.
-
+(*Inductive eventinform :=
+| Event : event -> eventinform
+| EBinop : (* What is the type of a register name? *)
+*)
 Definition cur_comp_of_event (e: event) : Component.id :=
   match e with
   | ECall  C _ _ _ => C
