Common/Blame.v
@@ -3,7 +3,7 @@ Require Import CompCert.Events.
 Require Import CompCert.Behaviors.
 From mathcomp Require Import ssreflect seq.
 
-Definition extract_finite_trace (beh: program_behavior) : option trace :=
+Definition extract_finite_trace {Ev: Type} (beh: program_behavior) : option (trace Ev) :=
   match beh with
   | Terminates t => Some t
   | Diverges t => Some t
@@ -11,8 +11,8 @@ Definition extract_finite_trace (beh: program_behavior) : option trace :=
   | Goes_wrong t => Some t
   end.
 
-Definition last_comp (t: trace) :=
+Definition last_comp {Ev} {evInst : EventClass Ev} (t: trace Ev) :=
   last Component.main [seq next_comp_of_event e | e <- t].
 
-Definition undef_in (t: trace) (iface: Program.interface) :=
+Definition undef_in {Ev} {evInst : EventClass Ev} (t: trace Ev) (iface: Program.interface) :=
   last_comp t \in domm iface.
